Some fixes to evm.lem

Hoare/TrTermination.thy
@@ -4,8 +4,38 @@ imports Balance
 
 begin
 
+definition vm_gas :: "instruction_result \<Rightarrow> int" where
+"vm_gas vm = (case vm of
+   InstructionContinue v \<Rightarrow> vctx_gas v
+ | InstructionToEnvironment (ContractCall args) v hint \<Rightarrow>
+    vctx_gas v + uint (callarg_gas args)
+ | InstructionToEnvironment (ContractDelegateCall args) v hint \<Rightarrow>
+    vctx_gas v + uint (callarg_gas args)
+ | InstructionToEnvironment _ v hint \<Rightarrow>
+    vctx_gas v
+ | _ \<Rightarrow> 0 )"
+
+definition stack_gas ::
+   "(world_state * variable_ctx * constant_ctx * stack_hint) list \<Rightarrow> nat \<Rightarrow> int" where
+"stack_gas lst i = (let (_,v,_,_) = lst!i in vctx_gas v)"
+
+definition system_gas :: "global0 \<Rightarrow> int" where
+"system_gas g =
+   vm_gas (g_vmstate g) + sum (stack_gas (g_stack g)) {0 .. length (g_stack g)}"
+
+lemma change_vmstate :
+  "g_stack st1 = g_stack st2 \<Longrightarrow>
+   vm_gas (g_vmstate st1) > vm_gas (g_vmstate st2) \<Longrightarrow>
+   system_gas st1 > system_gas st2"
+by (auto simp add:system_gas_def)
+
+lemma change_continue :
+  "vctx_gas v1 > vctx_gas v2 \<Longrightarrow>
+   vm_gas (InstructionContinue v1) > vm_gas (InstructionContinue v2)"
+by (auto simp add:vm_gas_def)
+
 (* basic case: simple instructions *)
-lemma basic :
+lemma basic_aux :
   "g_vmstate st1 = InstructionContinue v1 \<Longrightarrow>
    g_vmstate st2 = InstructionContinue v2 \<Longrightarrow>
    Continue st2 = next0 net (Continue st1) \<Longrightarrow>
@@ -23,6 +53,33 @@ by (simp add:next0_def next_state_def Let_def
   continue_meter_gas meter_gas_gt_0
   split:if_split_asm option.split_asm)
 
+lemma continue_stack :
+  "g_vmstate st1 = InstructionContinue v1 \<Longrightarrow>
+   g_vmstate st2 = InstructionContinue v2 \<Longrightarrow>
+   Continue st2 = next0 net (Continue st1) \<Longrightarrow>
+   g_stack st2 = g_stack st1"
+by (auto simp add:next0_def next_state_def Let_def
+  continue_meter_gas
+  split:if_split_asm option.split_asm list.split_asm
+   contract_action.split_asm stack_hint.split_asm)
+
+lemma basic :
+  "g_vmstate st1 = InstructionContinue v1 \<Longrightarrow>
+   g_vmstate st2 = InstructionContinue v2 \<Longrightarrow>
+   Continue st2 = next0 net (Continue st1) \<Longrightarrow>
+   Some inst = vctx_next_instruction v1 (g_cctx st1) \<Longrightarrow>
+   inst \<noteq> Misc STOP \<Longrightarrow>
+   inst \<noteq> Misc SUICIDE \<Longrightarrow>
+   inst \<noteq> Misc RETURN \<Longrightarrow>
+   inst \<noteq> Misc CALL \<Longrightarrow>
+   inst \<noteq> Misc CALLCODE \<Longrightarrow>
+   inst \<noteq> Misc DELEGATECALL \<Longrightarrow>
+   inst \<notin> range Unknown \<Longrightarrow>
+   vctx_memory_usage v1 \<ge> 0 \<Longrightarrow>
+   system_gas st1 > system_gas st2"
+using basic_aux change_continue change_vmstate continue_stack
+by force
+
 (* environment becomes a continue *)
 lemma env_continue :
   "g_vmstate st1 = InstructionToEnvironment act v1 hint \<Longrightarrow>
@@ -31,6 +88,180 @@ lemma env_continue :
 by (auto simp add:next0_def next_state_def Let_def
   split:if_split_asm option.split_asm list.split_asm
    contract_action.split_asm stack_hint.split_asm)
+
+lemma continue_meter :
+  "g_vmstate st1 = InstructionContinue v1 \<Longrightarrow>
+   g_vmstate st2 = InstructionContinue v2 \<Longrightarrow>
+   Continue st2 = next0 net (Continue st1) \<Longrightarrow>
+   Some inst = vctx_next_instruction v1 (g_cctx st1) \<Longrightarrow>
+   vctx_gas v2 = vctx_gas v1 - meter_gas inst v1 (g_cctx st1) net"
+by (auto simp add:next0_def next_state_def Let_def
+  continue_meter_gas
+  split:if_split_asm option.split_asm list.split_asm
+   contract_action.split_asm stack_hint.split_asm)
+
+
+
+lemma env_meter :
+  "g_vmstate st1 = InstructionContinue v1 \<Longrightarrow>
+   g_vmstate st2 = InstructionToEnvironment act v2 hint \<Longrightarrow>
+   Continue st2 = next0 net (Continue st1) \<Longrightarrow>
+   act \<notin> range ContractFail \<Longrightarrow>
+   Some inst = vctx_next_instruction v1 (g_cctx st1) \<Longrightarrow>
+   vctx_gas v2 = vctx_gas v1 - meter_gas inst v1 (g_cctx st1) net"
+by (auto simp add:next0_def next_state_def Let_def
+  env_meter_gas
+  split:if_split_asm option.split_asm list.split_asm
+   contract_action.split_asm stack_hint.split_asm)
+
+lemma call_to_env :
+"inst \<in> {Misc CALL, Misc CALLCODE, Misc DELEGATECALL} \<Longrightarrow>
+ \<exists>act v2 x33. instruction_sem v1 c inst net =
+ InstructionToEnvironment act v2 x33"
+apply (simp only: instruction_sem_def)
+  apply (case_tac inst; clarsimp)
+apply (case_tac x13 ; clarsimp simp: rw
+           split:list.splits)
+done
+
+lemmas split_inst = arith_inst.split_asm bits_inst.split_asm 
+  sarith_inst.split_asm
+  info_inst.split_asm
+  memory_inst.split_asm
+  storage_inst.split_asm
+  pc_inst.splits
+  stack_inst.split_asm
+  bits_inst.split_asm
+  log_inst.split_asm
+  bits_inst.split_asm
+  misc_inst.split_asm
+  inst.splits
+ list.splits option.splits if_splits
+
+lemma did_not_call :
+"inst \<notin> {Misc CALL, Misc CALLCODE} \<Longrightarrow>
+ instruction_sem v1 c inst net =
+ InstructionToEnvironment (ContractCall args) v2 x33 \<Longrightarrow>
+ False"
+by (auto simp:instruction_sem_simps Let_def split:split_inst)
+
+lemma did_not_delegate :
+"inst \<noteq> Misc DELEGATECALL \<Longrightarrow>
+ instruction_sem v1 c inst net =
+ InstructionToEnvironment (ContractDelegateCall args) v2 x33 \<Longrightarrow>
+ False"
+by (auto simp:instruction_sem_simps Let_def split:split_inst)
+
+lemma word_convert_compare : "x \<ge> 0 \<Longrightarrow> uint (word_of_int x) \<le> x"
+  by (simp add: int_word_uint zmod_le_nonneg_dividend)
+
+lemma cmem_new :
+ "memu \<ge> 0 \<Longrightarrow>
+  Cmem (new_memory_consumption
+    inst memu x21 x21a z x21c x21d x21e x21f)
+   \<ge> Cmem memu"
+  by (simp add: Cmem_lift vctx_memory_usage_never_decreases)
+
+lemma cmem_new_helper :
+ "memu \<ge> 0 \<Longrightarrow> k > 0 \<Longrightarrow>
+  0 < Cmem (new_memory_consumption
+    inst memu x21 x21a z x21c x21d x21e x21f) +
+   (k - Cmem memu)"
+using cmem_new
+proof -
+  assume a1: "0 \<le> memu"
+  assume "0 < k"
+  then have "\<not> k \<le> 0"
+    by (metis not_less)
+  then have "\<not> k \<le> Cmem memu - Cmem (new_memory_consumption inst memu x21 x21a z x21c x21d x21e x21f)"
+    using a1 by (meson cmem_new le_iff_diff_le_0 order.trans)
+  then show ?thesis
+    by linarith
+qed
+
+lemma cmem_new_helper2 :
+ "memu \<ge> 0 \<Longrightarrow> k > 0 \<Longrightarrow>
+  0 < k + (Cmem (new_memory_consumption
+    inst memu x21 x21a z x21c x21d x21e x21f) - Cmem memu)"
+  by (simp add: add_pos_nonneg cmem_new)
+
+lemma min_L :
+   "v1 < v2 \<Longrightarrow>
+    v1 > 0 \<Longrightarrow>
+     min (L (gs-v1)) x < min (L (gs-v2)) x + v2"
+by (auto simp add:L_def)
+
+lemma min_L_helper :
+   "v1 < v2 \<Longrightarrow>
+    v1 > 0 \<Longrightarrow>
+    memu \<ge> 0 \<Longrightarrow>
+     min (L (gs-v1-z)) x <
+    Cmem (new_memory_consumption
+    inst memu x21 x21a z12 x21c x21d x21e x21f) - Cmem memu
+    + (min (L (gs-v2-z)) x + v2)"
+using cmem_new [of memu inst x21 x21a z12 x21c x21d x21e x21f]
+  L_def
+by force
+
+lemma min_L_helper2 :
+   "v1 < v2 \<Longrightarrow>
+    v1 > 0 \<Longrightarrow>
+    memu \<ge> 0 \<Longrightarrow>
+    min (L (gs-v1-z)) x <
+    v2 + (Cmem (new_memory_consumption
+    inst memu x21 x21a z12 x21c x21d x21e x21f)
+    + (min (L (gs-v2-z)) x  - Cmem memu))"
+using cmem_new [of memu inst x21 x21a z12 x21c x21d x21e x21f]
+  L_def
+by force
+
+lemma call_gas_compare :
+"vctx_memory_usage v1 \<ge> 0 \<Longrightarrow>
+ vctx_recipient v1 c = ucast x21a \<Longrightarrow>
+ vctx_stack v1 = x21 # x21a # x21b # x21c # x21d # x21e # x21f # x22f \<Longrightarrow>
+ Ccallgas x21 x21a x21b (\<not> vctx_account_existence v1 (ucast x21a))
+                (vctx_gas v1) net
+                (calc_memu_extra (vctx_memory_usage v1) x21 x21a x21b x21c x21d x21e
+                  x21f)
+       < meter_gas (Misc CALL) v1 c net"
+by (auto simp add:gas_simps  Ccallgas_def meter_gas_def C_def
+  thirdComponentOfC_def Gcallstipend_def vctx_stack_default_def
+  uint_nat cmem_new_helper  cmem_new_helper2
+calc_memu_extra_def min_L_helper min_L_helper2)
+
+lemma memu_extra_ge0 :
+"memu \<ge> 0 \<Longrightarrow>
+ calc_memu_extra memu x21 x21a x21b x21c x21d x21e x21f \<ge> 0"
+by (simp add:calc_memu_extra_def cmem_new)
+
+lemma callgas_ge0 :
+  "memu \<ge> 0 \<Longrightarrow>
+   Ccallgas x21 x21a x21b aex gas1 net memu \<ge> 0"
+apply (auto simp add:gas_simps  Ccallgas_def meter_gas_def C_def
+  thirdComponentOfC_def Gcallstipend_def vctx_stack_default_def
+  cmem_new_helper  cmem_new_helper2
+calc_memu_extra_def min_L_helper min_L_helper2 L_def)
+
+lemma call_system_gas :
+"instruction_sem v1 c (Misc CALL) net =
+ InstructionToEnvironment (ContractCall args) v2 x33 \<Longrightarrow>
+ vctx_gas v1 > vctx_gas v2 + uint (callarg_gas args)"
+apply (auto simp:instruction_sem_simps Let_def split:split_inst)
+
+
+(* calls without value (do not increase gas) *)
+(*
+lemma call_no_value :
+  "g_vmstate st1 = InstructionToEnvironment (ContractCall args) v1 hint \<Longrightarrow>
+   Continue st2 = next0 net (Continue st1) \<Longrightarrow>
+   g_vmstate st2 = InstructionContinue v2 \<Longrightarrow>
+   vctx_gas v2 \<le> vctx_gas v1 + uint (callarg_gas args)"
+apply (auto simp add:next0_def next_state_def Let_def
+  split:if_split_asm option.split_asm list.split_asm
+   contract_action.split_asm stack_hint.split_asm)
+*)
+
+(* calls with value *)
 
 end
 
